slides 25-

----

## Definition

> formulas $F$ and $G$ are equivalent if $\mathcal{A}(F) = \mathcal{A}(G)  \>\forall\mathcal{A}$ and we then write $F \equiv G$

relevant equivalences:
- proof by contradiction: $A \rightarrow B \equiv \neg B \rightarrow A$

>$\vDash F\rightarrow G$ iff $F \vDash G$
>$\vDash F\leftrightarrow G$ iff $F \equiv G$

----

## Reductions between problems

validity and unsatisfiability:$$\begin{align*}F \text{ valid}\quad & \text{ iff} &\neg F \text{ unsatisfiable} \\ F \text{ unsatisfiable}\quad & \text{ iff} &\neg F \text{ valid} \end{align*}$$validity and consequence:$$\begin{align*}F \text{ valid}\quad & \text{ iff} & \top\vDash F \\ F\vDash G\quad & \text{ iff} & F\rightarrow G \text{ valid}\end{align*}$$validity and equivalence:$$\begin{align*}F \text{ valid}\quad & \text{ iff} & F \equiv \top \\ F \equiv G\quad & \text{ iff} & F \leftrightarrow G\text{ valid}\end{align*}$$

----

## Properties of Semantic Equivalence

- semantic equivalence is an **equivalence relation** between formulas
	- number of equivalence classes = number of different assignments = $2^{2^{n}}$
	- explanation: $2^n$ assignments that can each have one of $2$ values
- semantic equivalence is **closed under operators**: if $F_1 \equiv F_2$, $G_1 \equiv G_2$, then also 
	- $(F_1 \land G_1) \equiv (F_2 \land G_2)$
	- $(F_1 \lor G_1) \equiv (F_2 \lor G_2)$ 
	- $\neg F_1 \equiv \neg F_2$

both properties together make semantic equivalence a **congruence relation**!

----

## Replacement Theorem

>Let 
> 1. $F \equiv G$
> 2. $H$ be a formula with an occurrence of $F$ as a subformula
> 3. $H'$ be the result of replacing an arbitrary occurrence of $F$ in $H$ by $G$
> then: $H \equiv H'$
> #replacementtheorem

in essence: replacing by equivalent formula produces equivalent formula

proof: induction on structure of $H$

----

## Important equivalences

| name            | equivalence                                              |
| --------------- | -------------------------------------------------------- |
| #idempotence     | $F \land F \equiv F$                                   |
|                 | $F \lor F \equiv F$                                    |
| #commutativity   | $F \land G \equiv G \land F$                         |
|                 | $F \lor G \equiv G \lor F$                           |
| #associativity   | $(F \land G) \land H \equiv F \land (G \land H)$     |
|                 | $(F \lor G) \lor H \equiv F \lor (G \lor H)$         |
| #absorption      | $F \land (F \lor G) \equiv F$                          |
|                 | $F \lor (F \land G) \equiv F$                          |
| #distributivity  | $F \land (G \lor H) \equiv (F \land G) \lor (F \land H)$ |
|                 | $F \lor (G \land H) \equiv (F \lor G) \land (F \lor H)$  |
| double negation | $\neg\neg F \equiv F$                                    |
| #deMorganslaws | $\neg(F \land G) \equiv \neg F \lor \neg G)$             |
|                 | $\neg(F \lor G) \equiv \neg F \land \neg G)$             |
|        -         | $\neg\bot\equiv\top$                                     |
|        -         | $\neg\top\equiv\bot$                                     |
|         -        | $(\top\lor G) \equiv \top$                               |
|          -       | $(\top\land G) \equiv G$                                 |
|           -      | $(\bot \lor G) \equiv G$                                 |
|            -     | $(\bot \land G)\equiv\bot$                                                         |
